Update CfgOptimizations.thy
Main Lemma for dead variables elimination (work is still in progress to get rid of the remaining sorry statements)

BoogieLang/CfgOptimizations.thy
@@ -1,6 +1,15 @@
 theory CfgOptimizations
-  imports Boogie_Lang.Semantics Boogie_Lang.Util "../global_data"
+  imports Boogie_Lang.Semantics Boogie_Lang.Util
 begin
+
+subsection \<open>Definition loop induction hypothesis\<close>
+
+definition loop_ih_optimizations
+  where "loop_ih_optimizations A M \<Lambda> \<Gamma> \<Omega> G G' LoopHeader LoopHeader'  m' s' j \<equiv> 
+          \<forall>j' ns1'. ((j' \<le> j) \<longrightarrow> 
+                     (A,M,\<Lambda>,\<Gamma>,\<Omega>,G \<turnstile>(Inl LoopHeader, Normal ns1') -n\<rightarrow>^j' (m', s')) \<longrightarrow>
+         (\<forall>m1' s1'.( A,M,\<Lambda>,\<Gamma>,\<Omega>,G' \<turnstile>(Inl LoopHeader', Normal ns1') -n\<rightarrow>* (m1', s1')) \<longrightarrow> s1' \<noteq> Failure) \<longrightarrow>
+                     s' \<noteq> Failure)"
 
 subsection \<open>Global block and hybrid global block lemma definition\<close>
 
@@ -194,7 +203,7 @@ qed
 qed
 
 
-subsection \<open>Main lemmas\<close>
+subsection \<open>Main lemmas for block coalescing and pruning of unreachable blocks\<close>
 
 text \<open>In the following subsection, we show the two main lemmas that are interested in:
     \<^item> Given the hybrid global lemma for block i, we can construct the hybrid block lemma for block i-1 
@@ -418,7 +427,7 @@ proof (rule allI | rule impI)+
   qed
 qed
 
-text \<open>The following lemma shows that if in a block the global block lemma holds for all successors and the block was not coalesced, then the global block lemma holds\<close>
+subsubsection \<open>Main Lemma 3 (The following lemma shows that if in a block the global block lemma holds for all successors and the block was not coalesced, then the global block lemma holds)\<close>
 
 lemma global_block_succ:
   assumes SuccBlocks: "out_edges G ! src_block = ls" and
@@ -517,7 +526,7 @@ proof (rule allI | rule impI)+
   qed
 qed
 
-text \<open>The following lemma shows that if in a block the global block lemma holds for all successors and the block was coalesced, then the hybrid block lemma holds\<close>
+subsubsection \<open>Main Lemma 4: The following lemma shows that if in a block the global block lemma holds for all successors and the block was coalesced, then the hybrid block lemma holds\<close>
 
 lemma hybrid_block_succ:
   assumes SuccBlocks: "out_edges G ! src_block = ls" and
@@ -596,7 +605,7 @@ proof (rule allI | rule impI)+
 
 qed
 
-
+subsubsection \<open>Main Lemma 5: Following Lemma shows correctness of pruning of unreachable blocks if the block was not coalesced\<close>
 
 lemma pruning_not_coalesced:
   assumes SuccBlocks: "out_edges G ! src_block = ls" and
@@ -640,11 +649,12 @@ proof (rule allI | rule impI)+
   qed
 qed
 
+subsubsection \<open>Main Lemma 6: Following Lemma shows correctness of pruning of unreachable blocks if the block was coalesced\<close>
+
 lemma pruning_coalesced:
-  assumes SuccBlocks: "out_edges G ! src_block = ls" and
-          TargetBlock: "node_to_block G' ! tgt_block = tgt_cmds" and
+  assumes TargetBlock: "node_to_block G' ! tgt_block = tgt_cmds" and
           SourceBlock: "node_to_block G ! src_block = src_cmds" and
-          Pruning: "(Assert (Lit (LBool False))) \<in> set (src_cmds)" and
+          Pruning: "(Assert (Lit (LBool False))) \<in> set (src_cmds) \<or> (Assume (Lit (LBool False))) \<in> set (src_cmds)" and
           Coalesced: "tgt_cmds = cs@src_cmds"
         shows "hybrid_block_lemma A M \<Lambda> \<Gamma> \<Omega> G G' src_block tgt_block src_cmds"
   unfolding hybrid_block_lemma_def
@@ -664,7 +674,7 @@ proof (rule allI | rule impI)+
     proof (cases "(Assume (Lit (LBool False))) \<in> set (src_cmds)")
       case True
       have "A,M,\<Lambda>,\<Gamma>,\<Omega> \<turnstile> \<langle>src_cmds,Normal ns\<rangle> [\<rightarrow>] s'"
-        by (smt (verit) "2"(1) "2"(2) Inl_inject Pair_inject Pruning SourceBlock converse_rtranclpE magic_lemma_assert_false red_cfg.simps state.distinct(1) state.distinct(3))
+        by (smt (verit) "2"(1) "2"(2) Inl_inject Pair_inject SourceBlock True converse_rtranclpE magic_lemma_assume_false red_cfg.cases state.distinct(1) state.distinct(3))
       hence "s' = Magic"
         using TargetVerifies True hybrid_block_lemma_target_verifies_def magic_lemma_assume_false by blast
       then show ?thesis
@@ -672,16 +682,924 @@ proof (rule allI | rule impI)+
     next
       case False
       have "A,M,\<Lambda>,\<Gamma>,\<Omega> \<turnstile> \<langle>src_cmds,Normal ns\<rangle> [\<rightarrow>] s'"
-        by (smt (verit) "2"(1) "2"(2) Inl_inject Pair_inject Pruning SourceBlock converse_rtranclpE magic_lemma_assert_false red_cfg.simps state.distinct(1) state.distinct(3))
+        by (smt (verit) "2"(1) "2"(2) False Inl_inject Pair_inject Pruning SourceBlock converse_rtranclpE magic_lemma_assert_false red_cfg.cases state.distinct(1) state.distinct(3))
       hence "s' = Magic \<or> s' = Failure" using magic_lemma_assert_false Pruning 
-        by blast
+        using False by blast
       then show ?thesis using Coalesced RedFailure TargetBlock TargetVerifies \<open>A,M,\<Lambda>,\<Gamma>,\<Omega> \<turnstile> \<langle>src_cmds,Normal ns\<rangle> [\<rightarrow>] s'\<close>
         by (simp add: hybrid_block_lemma_target_verifies_def)
     qed
   qed
 qed
 
+subsection \<open>Definition of free variables\<close>
 
-term "global_data.fdecls"
+fun free_var_expr :: "expr \<Rightarrow> vname set"
+where 
+  "free_var_expr (Var n) = {n}"
+| "free_var_expr (BVar n) = {}"
+| "free_var_expr (Lit n) = {}"
+| "free_var_expr (UnOp unop ex) = free_var_expr (ex)"
+| "free_var_expr (BinOp ex1 binop ex2) = free_var_expr (ex1) \<union> free_var_expr (ex2)"
+| "free_var_expr (FunExp fname ty_list ex_ls)  = \<Union> (Set.image free_var_expr (set ex_ls))" 
+| "free_var_expr (Old ex) = free_var_expr (ex)"
+| "free_var_expr (Forall ty ex) = free_var_expr (ex)"
+| "free_var_expr (Exists ty ex) = free_var_expr (ex)"
+| "free_var_expr (ForallT ex) = free_var_expr (ex)"
+| "free_var_expr (ExistsT ex) = free_var_expr (ex)"
+
+fun free_var_exprlist :: "expr list \<Rightarrow> vname set"
+where
+  "free_var_exprlist cs = \<Union> (Set.image free_var_expr (set cs))"
+
+
+fun free_var_cmd :: "cmd \<Rightarrow> vname set"
+where
+  "free_var_cmd (Assert ex) = free_var_expr ex"
+| "free_var_cmd (Assume ex) = free_var_expr ex"
+| "free_var_cmd (Assign vname expr) = {vname} \<union> free_var_expr expr"
+| "free_var_cmd (Havoc vname) = {vname}"
+| "free_var_cmd (ProcCall pname ex_ls vname_ls) = set vname_ls \<union> (\<Union> (Set.image free_var_expr (set ex_ls)))" (* is this correct?" *)
+
+fun free_var_cmdlist :: "cmd list \<Rightarrow> vname set"
+where
+  "free_var_cmdlist cs = \<Union> (Set.image free_var_cmd (set cs))"
+
+subsection \<open>Helper Lemmas for the final dead variables elimination lemma\<close>
+
+lemma validConf:
+  assumes proc_cor: "proc_is_correct A fun_decls constants global_vars axioms proc Semantics.proc_body_satisfies_spec" and
+                    "proc_body proc = Some (locals, mbody)" and
+                    "(((\<forall>t. closed t \<longrightarrow> (\<exists>v. type_of_val A (v :: 'a val) = t)) \<and> (\<forall>v. closed ((type_of_val A) v))))" and
+                    "fun_interp_wf A fun_decls \<Gamma>" and
+                    "list_all closed \<Omega> \<and> length \<Omega> = proc_ty_args proc" and        
+                    "state_typ_wf A \<Omega> gs (constants @ global_vars)" and
+                    "state_typ_wf A \<Omega> ls ((proc_args proc)@ (locals @ proc_rets proc))" and
+                    "axioms_sat A (constants, []) \<Gamma> (global_to_nstate (state_restriction gs constants)) axioms" and            
+                    "expr_all_sat A (constants@global_vars, (proc_args proc)@(locals@(proc_rets proc))) \<Gamma> \<Omega> \<lparr>old_global_state = gs, global_state = gs, local_state = ls, binder_state = Map.empty\<rparr> (proc_all_pres proc)" and 
+                    "A, [], (constants@global_vars, (proc_args proc)@(locals@(proc_rets proc))), \<Gamma>, \<Omega>, mbody \<turnstile> (Inl (entry(mbody)), Normal \<lparr>old_global_state = gs, global_state = gs, local_state = ls, binder_state = Map.empty\<rparr>) -n\<rightarrow>* (m',s')"
+
+  shows             "valid_configuration A (constants@global_vars, (proc_args proc)@(locals@(proc_rets proc))) \<Gamma> \<Omega> (proc_checked_posts proc) m' s'"
+  using assms
+  unfolding proc_body_satisfies_spec_def
+  by fastforce
+
+lemma map_le_append_pre:
+  assumes "map_of xs \<subseteq>\<^sub>m map_of xs'"
+  shows "map_of (ys@xs) \<subseteq>\<^sub>m map_of (ys@xs')" 
+  using assms
+  by (metis Map.map_of_append append_assoc map_add_subsumed2 map_le_map_add)
+  
+lemma map_le_append_post:
+  assumes "map_of xs \<subseteq>\<^sub>m map_of xs'" and 
+          \<comment>\<open>This second assumption is necessary, because otherwise \<^term>\<open>map_of (xs@ys) y\<close> may lookup
+             a value in \<^term>\<open>ys\<close>, while \<^term>\<open>map_of (xs'@ys) y\<close> looks up the value in \<^term>\<open>xs'\<close>\<close>
+          "dom (map_of xs') \<inter> dom (map_of ys) = {}"
+  shows "map_of (xs@ys) \<subseteq>\<^sub>m map_of (xs'@ys)"
+  using assms
+  by (metis Map.map_of_append map_add_comm map_add_le_mapI map_le_map_add map_le_trans)
+
+lemma map_le_append_pre_post:
+  assumes "map_of xs \<subseteq>\<^sub>m map_of xs'" and 
+          \<comment>\<open>This second assumption is necessary, because otherwise \<^term>\<open>map_of (xs@ys) y\<close> may lookup
+             a value in \<^term>\<open>ys\<close>, while \<^term>\<open>map_of (xs'@ys) y\<close> looks up the value in \<^term>\<open>xs'\<close>\<close>
+          "dom (map_of xs') \<inter> dom (map_of ys) = {}"
+  shows "map_of (ws@xs@ys) \<subseteq>\<^sub>m map_of (ws@xs'@ys)"
+  using assms map_le_append_pre map_le_append_post
+  by blast 
+
+lemma lookup_var_decl_map_le:
+  assumes "map_of vs \<subseteq>\<^sub>m map_of vs'"          
+  shows "lookup_vdecls_ty vs \<subseteq>\<^sub>m lookup_vdecls_ty vs'"
+  unfolding lookup_vdecls_ty_def map_le_def
+proof 
+  fix a
+  assume "a \<in> dom (\<lambda>x. map_option fst (map_of vs x))"
+
+  thus "map_option fst (map_of vs a) = map_option fst (map_of vs' a)"
+    using assms
+    by (metis (full_types) domIff map_le_def option.map_disc_iff)
+qed
+
+text \<open>The following lemma should be helpful to prove that variables reduce to the same values in 
+      in the program with and without dead variables.\<close>
+lemma lookup_var_map_le_local:
+  assumes MapLeLocal: "(map_of (snd \<Lambda>) \<subseteq>\<^sub>m map_of (snd \<Lambda>') \<and> x \<notin> (dom (map_of (snd \<Lambda>')) - (dom (map_of (snd \<Lambda>))))) 
+                       \<or> (map_of (snd \<Lambda>') \<subseteq>\<^sub>m map_of (snd \<Lambda>) \<and> x \<notin> (dom (map_of (snd \<Lambda>)) - (dom (map_of (snd \<Lambda>'))))) "
+  shows "lookup_var \<Lambda> ns x = lookup_var \<Lambda>' ns x"
+proof (cases "(map_of (snd \<Lambda>) \<subseteq>\<^sub>m map_of (snd \<Lambda>') \<and> x \<notin> (dom (map_of (snd \<Lambda>')) - (dom (map_of (snd \<Lambda>)))))")
+  case True
+  then show ?thesis
+  proof (cases "map_of (snd \<Lambda>) x = None")
+    case True
+    hence "map_of (snd \<Lambda>') x = None"
+      by (metis (mono_tags, lifting) DiffI assms domIff map_le_def)
+    with True show ?thesis 
+      unfolding lookup_var_def
+      by simp
+  next
+    case False
+    then show ?thesis
+      using MapLeLocal
+      unfolding lookup_var_def
+      by (metis (mono_tags, lifting) True domIff map_le_def)
+  qed
+next
+  case False
+  then show ?thesis
+  proof (cases "map_of (snd \<Lambda>') x = None")
+    case True
+    hence "map_of (snd \<Lambda>) x = None"
+      using False assms by blast
+    with True show ?thesis 
+      unfolding lookup_var_def
+      by simp
+  next
+    case False
+    then show ?thesis 
+      using MapLeLocal
+      unfolding lookup_var_def
+      by (metis (mono_tags, lifting) DiffI domIff map_le_def)
+  qed
+qed
+
+
+lemma binder_map_le_local:
+  assumes MapLeLocal: "map_of (snd \<Lambda>) \<subseteq>\<^sub>m map_of (snd \<Lambda>')" and
+          "x \<notin> (dom (map_of (snd \<Lambda>')) - (dom (map_of (snd \<Lambda>))))"
+        shows "binder_state ns i = binder_state ns i"
+  by simp
+
+
+
+lemma state_typ_wf_map_le:
+  assumes StateTypWf: "state_typ_wf A \<Omega> ls (proc_args proc @ locals' @ proc_rets proc)" (is "state_typ_wf A \<Omega> ls ?V'") and
+         MapLe: "map_of locals \<subseteq>\<^sub>m map_of locals'" and
+         DomLocalInterRetsEmpty:   "dom (map_of locals') \<inter> dom (map_of (proc_rets proc)) = {}"
+        shows "state_typ_wf A \<Omega> ls (proc_args proc @ locals @ proc_rets proc)" (is "state_typ_wf A \<Omega> ls ?V")
+  unfolding state_typ_wf_def
+proof (rule allI | rule impI)+
+  fix v t
+  assume LookupV: "lookup_vdecls_ty (proc_args proc @ locals @ proc_rets proc) v = Some t"
+
+  from MapLe have "map_of ?V \<subseteq>\<^sub>m map_of ?V'"
+    using map_le_append_pre_post[OF MapLe DomLocalInterRetsEmpty]
+    by blast        
+
+  with LookupV
+  have "lookup_vdecls_ty (proc_args proc @ locals' @ proc_rets proc) v = Some t"
+    using lookup_var_decl_map_le
+    by (metis (full_types) domI map_le_def)
+
+  thus "map_option (type_of_val A) (ls v) = Some (instantiate \<Omega> t)"
+    using StateTypWf
+    unfolding state_typ_wf_def
+    by blast
+qed
+
+
+
+
+lemma expr_eval_different_locals_same_value:
+  assumes  "fst \<Lambda> = fst \<Lambda>'" and
+           "map_of (snd \<Lambda>') \<subseteq>\<^sub>m map_of (snd \<Lambda>)  \<or> map_of (snd \<Lambda>) \<subseteq>\<^sub>m map_of (snd \<Lambda>')" 
+  shows    "A,\<Lambda>,\<Gamma>,\<Omega> \<turnstile> \<langle>e, s\<rangle> \<Down> v \<Longrightarrow> 
+              free_var_expr e \<inter> ((dom (map_of (snd \<Lambda>')) - dom (map_of (snd \<Lambda>))) \<union> (dom (map_of (snd \<Lambda>)) - dom (map_of (snd \<Lambda>')))) = {} 
+              \<Longrightarrow> A,\<Lambda>',\<Gamma>,\<Omega> \<turnstile> \<langle>e, s\<rangle> \<Down> v" and
+           "A,\<Lambda>,\<Gamma>,\<Omega> \<turnstile> \<langle>es, s\<rangle> [\<Down>] vs \<Longrightarrow>
+              \<Union> {free_var_expr e' | e'. e' \<in> set es} \<inter> ((dom (map_of (snd \<Lambda>')) - dom (map_of (snd \<Lambda>))) \<union> (dom (map_of (snd \<Lambda>)) - dom (map_of (snd \<Lambda>')))) = {} 
+              \<Longrightarrow> A,\<Lambda>',\<Gamma>,\<Omega> \<turnstile> \<langle>es, s\<rangle> [\<Down>] vs"
+  using assms
+proof (induction rule: red_expr_red_exprs.inducts)
+  case (RedVar n_s x v \<Omega>)
+  then show ?case
+  proof (cases "map_of (snd \<Lambda>') \<subseteq>\<^sub>m map_of (snd \<Lambda>)")
+    case True
+    have "free_var_expr (Var x) \<inter> (dom (map_of (snd \<Lambda>)) - (dom (map_of (snd \<Lambda>')))) = {}"
+      using RedVar.prems(1)
+      by blast
+
+    hence notin: "x \<notin> (dom (map_of (snd \<Lambda>)) - (dom (map_of (snd \<Lambda>'))))"
+      using Int_Un_eq(2) RedVar.prems(1) by auto
+
+    have "lookup_var \<Lambda>' n_s x = lookup_var \<Lambda> n_s x"
+      apply (rule lookup_var_map_le_local)
+      using True notin by auto
+
+    then show ?thesis
+      by (simp add: RedVar.IH red_expr_red_exprs.RedVar)
+  next
+    case False
+
+    have "free_var_expr (Var x) \<inter> (dom (map_of (snd \<Lambda>')) - (dom (map_of (snd \<Lambda>)))) = {}"
+      using RedVar.prems(1)
+      by blast
+
+    hence notin: "x \<notin> (dom (map_of (snd \<Lambda>')) - (dom (map_of (snd \<Lambda>))))"
+      by simp
+
+    have "lookup_var \<Lambda>' n_s x = lookup_var \<Lambda> n_s x"
+      apply (rule lookup_var_map_le_local)
+      using False notin assms(2) by blast
+
+    then show ?thesis
+      by (simp add: RedVar.IH red_expr_red_exprs.RedVar)
+  qed
+next
+  case (RedBVar n_s i v \<Omega>)
+  then show ?case
+    by (simp add: red_expr_red_exprs.RedBVar)
+next
+  case (RedLit \<Omega> v n_s)
+  then show ?case
+    by (simp add: red_expr_red_exprs.RedLit)
+next
+  case (RedBinOp \<Omega> e1 n_s v1 e2 v2 bop v)
+
+
+  have v1: "A,\<Lambda>',\<Gamma>,\<Omega> \<turnstile> \<langle>e1,n_s\<rangle> \<Down> v1"
+    by (metis (no_types, lifting) Diff_Compl Int_Diff Int_empty_right RedBinOp.IH(2) RedBinOp.prems(1) RedBinOp.prems(3) Un_Int_eq(3) assms(1) free_var_expr.simps(5))
+
+  have v2: "A,\<Lambda>',\<Gamma>,\<Omega> \<turnstile> \<langle>e2,n_s\<rangle> \<Down> v2"
+    using RedBinOp.IH(4) RedBinOp.prems(1) RedBinOp.prems(3) assms(1) free_var_expr.simps(5) by blast
+  show ?case
+    using v1 v2
+    using RedBinOp.hyps red_expr_red_exprs.RedBinOp by blast
+next
+  case (RedUnOp \<Omega> e n_s v uop v')
+  then show ?case
+    by (simp add: red_expr_red_exprs.RedUnOp)
+next
+  case (RedFunOp f f_interp \<Omega> args n_s v_args ty_args v)
+
+
+  have "\<Union> {free_var_expr e' |e'. e' \<in> set args} \<inter> ((dom (map_of (snd \<Lambda>')) - dom (map_of (snd \<Lambda>))) \<union> (dom (map_of (snd \<Lambda>)) - dom (map_of (snd \<Lambda>')))) = {}"
+    using RedFunOp.prems(1) free_var_expr.simps(6)
+    by blast
+
+  hence "A,\<Lambda>',\<Gamma>,\<Omega> \<turnstile> \<langle>args, n_s\<rangle> [\<Down>] v_args"
+    by (simp add: RedFunOp.IH(3) RedFunOp.prems(3) assms(1))
+
+  then show ?case
+    using RedFunOp
+    by (simp add: red_expr_red_exprs.RedFunOp)
+next
+(*case (RedCondExpTrue \<Omega> cond n_s thn v els)
+  then show ?case sorry
+next
+  case (RedCondExpFalse \<Omega> cond n_s els v thn)
+  then show ?case sorry
+next *)
+  case (RedOld \<Omega> e n_s v)
+  then show ?case
+    by (simp add: red_expr_red_exprs.RedOld)
+next
+  case (RedExpListNil \<Omega> n_s)
+  then show ?case
+    by (meson red_expr_red_exprs.RedExpListNil)
+next
+  case (RedExpListCons \<Omega> e n_s v es vs)
+
+  have free_var_e: "free_var_expr e \<inter> ((dom (map_of (snd \<Lambda>')) - dom (map_of (snd \<Lambda>))) \<union> (dom (map_of (snd \<Lambda>)) - dom (map_of (snd \<Lambda>')))) = {}"
+    using RedExpListCons.prems(1) by auto
+
+  then have expr: "A,\<Lambda>',\<Gamma>,\<Omega> \<turnstile> \<langle>e,n_s\<rangle> \<Down> v"
+    by (simp add: RedExpListCons.IH(2) RedExpListCons.prems(3) assms(1))
+
+  have "\<Union> {free_var_expr e' |e'. e' \<in> set es} \<subseteq> \<Union> {free_var_expr e' |e'. e' \<in> set (e # es)}"
+    by auto
+
+  then have "\<Union> {free_var_expr e' |e'. e' \<in> set es} \<inter> ((dom (map_of (snd \<Lambda>')) - dom (map_of (snd \<Lambda>))) \<union> (dom (map_of (snd \<Lambda>)) - dom (map_of (snd \<Lambda>')))) = {}"
+    using RedExpListCons.prems(1) boolean_algebra_cancel.inf1 inf.absorb_iff1 inf_bot_right by blast
+
+  then have expr: "A,\<Lambda>',\<Gamma>,\<Omega> \<turnstile> \<langle>es,n_s\<rangle> [\<Down>] vs"
+    by (simp add: RedExpListCons.IH(4) RedExpListCons.prems(3) assms(1))
+  then show ?case
+    using expr
+    by (simp add: RedExpListCons.IH(2) RedExpListCons.prems(3) assms(1) free_var_e red_expr_red_exprs.RedExpListCons)
+next
+  case (RedForAllTrue \<Omega> ty e n_s)
+  then show ?case
+    by (simp add: red_expr_red_exprs.RedForAllTrue)
+next
+  case (RedForAllFalse v \<Omega> ty e n_s)
+  then show ?case
+    using free_var_expr.simps(8) red_expr_red_exprs.RedForAllFalse by blast
+next
+  case (RedExistsTrue v \<Omega> ty e n_s)
+  then show ?case
+    using free_var_expr.simps(9) red_expr_red_exprs.RedExistsTrue by blast
+next
+  case (RedExistsFalse \<Omega> ty e n_s)
+  then show ?case
+    by (simp add: red_expr_red_exprs.RedExistsFalse)
+next
+  case (RedForallT_True \<Omega> e n_s)
+  then show ?case
+    by (simp add: inf_set_def red_expr_red_exprs.RedForallT_True)
+next
+  case (RedForallT_False \<tau> \<Omega> e n_s)
+  then show ?case
+    by (simp add: red_expr_red_exprs.RedForallT_False)
+next
+  case (RedExistsT_True \<tau> \<Omega> e n_s)
+  then show ?case
+    by (simp add: red_expr_red_exprs.RedExistsT_True)
+next
+  case (RedExistsT_False \<Omega> e n_s)
+  then show ?case
+    by (simp add: red_expr_red_exprs.RedExistsT_False)
+qed
+
+
+
+lemma expr_sat_locals_same_value:
+  assumes ExprSat: "fst \<Lambda> = fst \<Lambda>'" and
+                   "(map_of (snd \<Lambda>) \<subseteq>\<^sub>m map_of (snd \<Lambda>') \<and> free_var_expr e \<inter> ((dom (map_of (snd \<Lambda>'))) - (dom (map_of (snd \<Lambda>)))) = {}) 
+                    \<or> (map_of (snd \<Lambda>') \<subseteq>\<^sub>m map_of (snd \<Lambda>) \<and> free_var_expr e \<inter> ((dom (map_of (snd \<Lambda>))) - (dom (map_of (snd \<Lambda>')))) = {})" 
+                   "expr_sat A \<Lambda> \<Gamma> \<Omega> s e"
+                 shows "expr_sat A \<Lambda>' \<Gamma> \<Omega> s e"
+  unfolding expr_sat_def
+  apply (rule expr_eval_different_locals_same_value[where ?\<Lambda> = "\<Lambda>"])
+     apply (simp add: ExprSat)
+  using assms(2) apply auto[1]
+  using assms(3) expr_sat_def apply blast
+  by (metis Diff_eq_empty_iff Int_Un_distrib Int_empty_right Un_empty_right assms(2) map_le_implies_dom_le)
+  
+
+
+
+
+
+
+
+
+lemma expr_sat_dead_variables:
+  assumes ExprSat: "expr_sat A (constants @ global_vars, proc_args proc @ locals @ proc_rets proc) \<Gamma> \<Omega> 
+                   ns expr" and
+          NoDeadVariables: "(map_of (proc_args proc @ locals @ proc_rets proc) \<subseteq>\<^sub>m map_of (proc_args proc @ locals' @ proc_rets proc) \<and> free_var_expr expr \<inter> (dom (map_of (proc_args proc @ locals' @ proc_rets proc))) - (dom (map_of (proc_args proc @ locals @ proc_rets proc))) = {}) 
+                           \<or> (map_of (proc_args proc @ locals' @ proc_rets proc) \<subseteq>\<^sub>m map_of (proc_args proc @ locals @ proc_rets proc) \<and> free_var_expr expr \<inter> (dom (map_of (proc_args proc @ locals @ proc_rets proc))) - (dom (map_of (proc_args proc @ locals' @ proc_rets proc))) = {})"
+
+shows "expr_sat A (constants @ global_vars, proc_args proc @ locals' @ proc_rets proc) \<Gamma> \<Omega> ns expr"
+  apply (rule expr_sat_locals_same_value[where ?\<Lambda> = "(constants @ global_vars, proc_args proc @ locals @ proc_rets proc)"])
+    apply simp
+  using NoDeadVariables
+   apply simp
+  using ExprSat by auto
+
+
+
+
+  
+
+
+lemma expr_list_sat_dead_variables:
+  assumes ExprSat: "expr_all_sat A (constants @ global_vars, proc_args proc @ locals @ proc_rets proc) \<Gamma> \<Omega> ns expr_list" and
+          MapLocal: "(map_of locals \<subseteq>\<^sub>m map_of locals' \<and> dom (map_of locals') \<inter> dom (map_of (proc_rets proc)) = {} \<and> free_var_exprlist expr_list \<inter> (dom (map_of (locals'))) - (dom (map_of (locals))) = {}) 
+                     \<or> (map_of locals' \<subseteq>\<^sub>m map_of locals \<and> dom (map_of locals) \<inter> dom (map_of (proc_rets proc)) = {} \<and> free_var_exprlist expr_list \<inter> (dom (map_of (locals))) - (dom (map_of (locals'))) = {})"
+
+shows "expr_all_sat A (constants @ global_vars, proc_args proc @ locals' @ proc_rets proc) \<Gamma> \<Omega> ns expr_list"
+  unfolding expr_all_sat_def list_all_def Ball_def
+proof (rule allI | rule impI)+
+  fix x
+  assume "x \<in> set (expr_list)"
+  show "expr_sat A (constants @ global_vars, proc_args proc @ locals' @ proc_rets proc) \<Gamma> \<Omega>
+          ns x"
+  proof (cases "map_of locals \<subseteq>\<^sub>m map_of locals'")
+    case True
+    have "dom (map_of locals') \<inter> dom (map_of (proc_rets proc)) = {}"
+      by (metis MapLocal True map_le_antisym)
+
+    have freeVarList: "free_var_exprlist expr_list \<inter> (dom (map_of (locals'))) - (dom (map_of (locals))) = {}"
+      by (metis MapLocal True map_le_antisym)
+
+    hence "free_var_exprlist expr_list \<inter> (dom (map_of (proc_args proc @ locals' @ proc_rets proc))) - (dom (map_of (proc_args proc @ locals @ proc_rets proc))) = {}"
+      by auto
+
+    hence freeVar: "free_var_expr x \<inter> (dom (map_of (proc_args proc @ locals' @ proc_rets proc))) - (dom (map_of (proc_args proc @ locals @ proc_rets proc))) = {}"
+      using \<open>x \<in> set expr_list\<close> free_var_exprlist.simps
+      by (simp add: Int_Diff Sup_inf_eq_bot_iff) 
+
+
+    have exprSat: "expr_sat A (constants @ global_vars, proc_args proc @ locals @ proc_rets proc) \<Gamma> \<Omega> ns x"
+      using ExprSat
+      unfolding expr_all_sat_def list_all_def Ball_def
+      by (simp add: \<open>x \<in> set expr_list\<close>)
+
+    have MapLe: "map_of (proc_args proc @ locals @ proc_rets proc) \<subseteq>\<^sub>m map_of (proc_args proc @ locals' @ proc_rets proc)"
+      by (metis MapLocal True map_le_antisym map_le_append_pre_post)
+    
+    
+    show ?thesis
+      apply (rule expr_sat_dead_variables)
+       apply (rule exprSat)
+      using MapLe freeVar by blast
+  next
+    case False
+
+    have exprSat: "expr_sat A (constants @ global_vars, proc_args proc @ locals @ proc_rets proc) \<Gamma> \<Omega> ns x"
+       using ExprSat
+       unfolding expr_all_sat_def list_all_def Ball_def
+       by (simp add: \<open>x \<in> set expr_list\<close>)
+    have map_of: "map_of (proc_args proc @ locals' @ proc_rets proc) \<subseteq>\<^sub>m map_of (proc_args proc @ locals @ proc_rets proc)"
+      using False MapLocal map_le_append_pre_post by blast
+
+    have domain: "dom (map_of locals) \<inter> dom (map_of (proc_rets proc)) = {}"
+      using False MapLocal by auto
+
+    have freeVarList: "free_var_exprlist expr_list \<inter> (dom (map_of (locals))) - (dom (map_of (locals'))) = {}"
+      by (metis MapLocal False)
+
+    hence "free_var_exprlist expr_list \<inter> (dom (map_of (proc_args proc @ locals @ proc_rets proc))) - (dom (map_of (proc_args proc @ locals' @ proc_rets proc))) = {}"
+      by auto
+
+    hence freeVar: "free_var_expr x \<inter> (dom (map_of (proc_args proc @ locals @ proc_rets proc))) - (dom (map_of (proc_args proc @ locals' @ proc_rets proc))) = {}"
+      using \<open>x \<in> set expr_list\<close> free_var_exprlist.simps
+      by (simp add: Int_Diff Union_disjoint)
+
+
+    show ?thesis 
+      apply (rule expr_sat_dead_variables[where ?locals = "locals"])
+       apply (rule exprSat)
+      using map_of freeVar by blast
+  qed
+qed
+
+lemma dom_diff_empty: 
+  assumes "A \<subseteq> B"
+  shows "A - B = {}"
+  by (simp add: assms)
+
+lemma red_cfg_dead_variables_cmd:
+  assumes "A,[],\<Lambda>',\<Gamma>,\<Omega> \<turnstile> \<langle>c,s\<rangle> \<rightarrow> s'" and
+          "fst \<Lambda> = fst \<Lambda>'" and
+          MapLocal: "(map_of (snd \<Lambda>) \<subseteq>\<^sub>m map_of (snd \<Lambda>'))" and
+          "free_var_cmd c \<inter> ((dom (map_of (snd \<Lambda>'))) - (dom (map_of (snd \<Lambda>)))) = {}" and
+          WhereClausesFreeVars: "\<And>x d cond. lookup_var_decl \<Lambda>' x = Some d \<Longrightarrow> snd d = Some cond \<Longrightarrow> free_var_expr cond \<inter> ((dom (map_of (snd \<Lambda>'))) - (dom (map_of (snd \<Lambda>)))) = {} "
+        shows "A,[],\<Lambda>,\<Gamma>,\<Omega> \<turnstile> \<langle>c,s\<rangle> \<rightarrow> s'"
+  using assms
+proof (induction rule: red_cmd.inducts)
+  case (RedAssertOk e n_s)
+  have "A,\<Lambda>,\<Gamma>,\<Omega> \<turnstile> \<langle>e,n_s\<rangle> \<Down> BoolV True"
+    apply (rule expr_eval_different_locals_same_value[where ?\<Lambda>=\<Lambda>'])
+    apply (simp add: assms(2))
+    apply (simp add: RedAssertOk.prems(2))
+    apply (simp add: RedAssertOk.hyps)
+    by (metis Diff_mono RedAssertOk.prems(2) RedAssertOk.prems(3) Un_absorb1 free_var_cmd.simps(1) map_le_implies_dom_le)
+  then show ?case
+    by (meson red_cmd.RedAssertOk)
+next
+  case (RedAssertFail e n_s)
+  have "A,\<Lambda>,\<Gamma>,\<Omega> \<turnstile> \<langle>e,n_s\<rangle> \<Down> BoolV False"
+    apply (rule expr_eval_different_locals_same_value[where ?\<Lambda>=\<Lambda>'])
+    apply (simp add: assms(2))
+    apply (simp add: RedAssertFail.prems(2))
+    apply (simp add: RedAssertFail.hyps)
+    by (metis Diff_mono RedAssertFail.prems(2) RedAssertFail.prems(3) Un_absorb1 free_var_cmd.simps(1) map_le_implies_dom_le)
+  then show ?case
+    by (meson red_cmd.RedAssertFail)
+next
+  case (RedAssumeOk e n_s)
+  have "A,\<Lambda>,\<Gamma>,\<Omega> \<turnstile> \<langle>e,n_s\<rangle> \<Down> BoolV True"
+    apply (rule expr_eval_different_locals_same_value[where ?\<Lambda>=\<Lambda>'])
+    apply (simp add: assms(2))
+    apply (simp add: RedAssumeOk.prems(2))
+    apply (simp add: RedAssumeOk.hyps)
+    by (metis Diff_eq_empty_iff RedAssumeOk.prems(2) RedAssumeOk.prems(3) boolean_algebra.disj_zero_right free_var_cmd.simps(2) map_le_implies_dom_le sup_commute)
+  then show ?case
+    by (meson red_cmd.RedAssumeOk)
+next
+  case (RedAssumeMagic e n_s)
+  have "A,\<Lambda>,\<Gamma>,\<Omega> \<turnstile> \<langle>e,n_s\<rangle> \<Down> BoolV False"
+    apply (rule expr_eval_different_locals_same_value[where ?\<Lambda>=\<Lambda>'])
+    apply (simp add: assms(2))
+    apply (simp add: RedAssumeMagic.prems(2))
+    apply (simp add: RedAssumeMagic.hyps)
+    by (metis Diff_eq_empty_iff RedAssumeMagic.prems(2) RedAssumeMagic.prems(3) boolean_algebra.disj_zero_right free_var_cmd.simps(2) map_le_implies_dom_le sup_commute)
+  then show ?case
+    by (meson red_cmd.RedAssumeMagic)
+next
+  case (RedAssign x ty v e n_s)
+  hence "x \<notin> (dom (map_of (snd \<Lambda>')) - dom (map_of (snd \<Lambda>)))"
+    by simp
+
+  hence "lookup_var_ty \<Lambda> x  = lookup_var_ty \<Lambda>' x"
+    unfolding lookup_var_ty_def lookup_var_decl_def
+    using assms
+    by (metis (no_types, lifting) DiffI domIff map_le_def)
+
+    
+  then have lookupEq: "lookup_var_ty \<Lambda> x = Some ty"
+    by (simp add: RedAssign.hyps(1))
+
+  have otherDirEmpty: "(dom (map_of (snd \<Lambda>)) - dom (map_of (snd \<Lambda>'))) = {}"
+    apply (rule dom_diff_empty)
+    using assms
+    by (simp add: map_le_implies_dom_le)
+
+  have "A,\<Lambda>,\<Gamma>,\<Omega> \<turnstile> \<langle>e, n_s\<rangle> \<Down> v"
+    apply (rule expr_eval_different_locals_same_value[where ?\<Lambda>=\<Lambda>'])
+    apply (simp add: assms(2))
+    apply (simp add: RedAssign.prems(2))
+    apply (simp add: RedAssign.hyps)
+    using RedAssign(6) MapLocal
+    unfolding free_var_cmd.simps
+    by (metis Int_Un_eq(2) Int_commute otherDirEmpty disjoint_insert(2) insert_is_Un)
+
+
+  then have step: "A,[],\<Lambda>,\<Gamma>,\<Omega> \<turnstile> \<langle>Assign x e,Normal n_s\<rangle> \<rightarrow> Normal (update_var \<Lambda> n_s x v)"
+    using lookupEq RedAssign.hyps(2) RedAssign
+    by (meson red_cmd.RedAssign)
+
+  have "(update_var \<Lambda> n_s x v) = (update_var \<Lambda>' n_s x v)"
+    unfolding update_var_def
+    using assms
+    by (smt (verit) Int_iff RedAssign.prems(3) Un_Diff_Int Un_iff domIff free_var_cmd.simps(3) insertCI insert_absorb insert_not_empty map_le_def)
+  then show ?case
+    using step by auto
+next
+  case (RedHavocNormal x ty w v n_s)
+
+  hence "x \<notin> (dom (map_of (snd \<Lambda>')) - dom (map_of (snd \<Lambda>)))"
+    by simp
+
+  hence lookupVarEq: "lookup_var_decl \<Lambda> x = lookup_var_decl \<Lambda>' x"
+    unfolding lookup_var_ty_def lookup_var_decl_def
+    using assms
+    by (metis (no_types, lifting) Diff_iff domIff map_le_def)
+
+  have otherDirEmpty: "(dom (map_of (snd \<Lambda>)) - dom (map_of (snd \<Lambda>'))) = {}"
+    apply (rule dom_diff_empty)
+    using assms
+    by (simp add: map_le_implies_dom_le)
+
+  have updVarEq:"(update_var \<Lambda> n_s x v) = (update_var \<Lambda>' n_s x v)"
+    unfolding update_var_def
+    using assms
+    by (smt (verit) Diff_Diff_Int Int_Diff Int_Diff_disjoint Int_insert_left RedHavocNormal.prems(3) Un_Diff_Int domIff free_var_cmd.simps(4) insert_disjoint(1) map_le_def)
+
+  have step: "\<And>cond. w = Some cond \<Longrightarrow> A,\<Lambda>,\<Gamma>,\<Omega> \<turnstile> \<langle>cond, (update_var \<Lambda> n_s x v)\<rangle> \<Down> BoolV True"
+  proof -
+    fix cond
+    assume "w = Some cond"
+    hence "free_var_expr cond \<inter> (dom (map_of (snd \<Lambda>')) - dom (map_of (snd \<Lambda>))) = {}"
+      using RedHavocNormal.hyps(1) WhereClausesFreeVars by auto
+    show "A,\<Lambda>,\<Gamma>,\<Omega> \<turnstile> \<langle>cond, (update_var \<Lambda> n_s x v)\<rangle> \<Down> BoolV True"
+      apply (rule expr_eval_different_locals_same_value[where ?\<Lambda>=\<Lambda>'])
+      apply (simp add: assms(2))
+      apply (simp add: RedHavocNormal.prems(2))
+      using RedHavocNormal.hyps(3)[OF \<open>w = Some cond\<close>]
+      apply (simp add: updVarEq)
+      by (simp add: \<open>free_var_expr cond \<inter> (dom (map_of (snd \<Lambda>')) - dom (map_of (snd \<Lambda>))) = {}\<close> otherDirEmpty)
+  qed
+
+
+  have "(update_var \<Lambda> n_s x v) = (update_var \<Lambda>' n_s x v)"
+    unfolding update_var_def
+    using assms
+    by (smt (verit) Diff_Diff_Int Diff_disjoint Diff_empty Diff_insert Diff_triv Int_insert_left Int_insert_right RedHavocNormal.hyps(1) RedHavocNormal.prems(2) RedHavocNormal.prems(3) domIff free_var_cmd.simps(4) insert_Diff_if insert_Diff_single insert_disjoint(1) insert_dom insert_inter_insert lookup_var_decl_local_2 map_le_def)
+
+
+  then show ?case
+    using updVarEq RedHavocNormal
+    by (metis local.step lookupVarEq red_cmd.RedHavocNormal)
+next
+  case (RedHavocMagic x ty cond v n_s)
+  have temp1: "lookup_var_decl \<Lambda> x = Some (ty,Some(cond))"
+    unfolding lookup_var_ty_def lookup_var_decl_def
+    using assms
+    by (metis (no_types, lifting) Int_Diff Int_insert_left_if1 RedHavocMagic.hyps(1) RedHavocMagic.prems(3) domIff free_var_cmd.simps(4) insert_Diff_if insert_not_empty lookup_var_decl_def map_le_def)
+
+  have updateEqual: "(update_var \<Lambda> n_s x v) = (update_var \<Lambda>' n_s x v)"
+    unfolding update_var_def
+    using assms
+    by (smt (verit) Diff_Diff_Int Diff_disjoint Diff_empty Diff_insert Diff_triv Int_insert_left Int_insert_right RedHavocMagic.hyps(1) RedHavocMagic.prems(2) RedHavocMagic.prems(3) domIff free_var_cmd.simps(4) insert_Diff_if insert_Diff_single insert_disjoint(1) insert_dom insert_inter_insert lookup_var_decl_local_2 map_le_def)
+
+  have otherDirEmpty: "(dom (map_of (snd \<Lambda>)) - dom (map_of (snd \<Lambda>'))) = {}"
+    apply (rule dom_diff_empty)
+    using assms
+    by (simp add: map_le_implies_dom_le)
+  
+  have "A,\<Lambda>,\<Gamma>,\<Omega> \<turnstile> \<langle>cond, (update_var \<Lambda> n_s x v)\<rangle> \<Down> BoolV False"
+    apply (rule expr_eval_different_locals_same_value[where ?\<Lambda>=\<Lambda>'])
+    apply (simp add: assms(2))
+    apply (simp add: RedHavocMagic.prems(2))
+    using updateEqual RedHavocMagic.hyps(3) apply simp
+    using assms RedHavocMagic otherDirEmpty
+    by (metis Int_Un_eq(2) snd_eqD)
+
+    
+  then show ?case 
+    using RedHavocMagic.hyps(2) red_cmd.RedHavocMagic temp1 by blast
+next
+  case (RedProcCallOkAndMagic m msig args n_s v_args pre_ls new_ls ty_modifs vs_modifs vs_ret post_ls post_gs post_state post_success post_fail n_s' rets)
+  then show ?case 
+    by simp
+next
+  case (RedProcCallFail m msig args n_s v_args pre_ls new_ls rets)
+  then show ?case 
+    by simp
+next
+  case (RedPropagateMagic s)
+  then show ?case
+    by (simp add: red_cmd.RedPropagateMagic)
+next
+  case (RedPropagateFailure s)
+  then show ?case
+    by (simp add: red_cmd.RedPropagateFailure)
+qed
+  
+
+lemma red_cfg_dead_variables_cmdlist:
+assumes "A,[],\<Lambda>',\<Gamma>,\<Omega> \<turnstile> \<langle>cs,s\<rangle> [\<rightarrow>] s'" and
+        "fst \<Lambda> = fst \<Lambda>'" and
+        MapLocal: "(map_of (snd \<Lambda>) \<subseteq>\<^sub>m map_of (snd \<Lambda>'))" and 
+        "free_var_cmdlist cs \<inter> ((dom (map_of (snd \<Lambda>'))) - (dom (map_of (snd \<Lambda>)))) = {}" and 
+        WhereClausesFreeVars: "\<And>x d cond. lookup_var_decl \<Lambda>' x = Some d \<Longrightarrow> snd d = Some cond \<Longrightarrow> free_var_expr cond \<inter> ((dom (map_of (snd \<Lambda>'))) - (dom (map_of (snd \<Lambda>)))) = {} "
+      shows "A,[],\<Lambda>,\<Gamma>,\<Omega> \<turnstile> \<langle>cs,s\<rangle> [\<rightarrow>] s'"
+  using assms
+proof (induction rule: red_cmd_list.inducts)
+  case (RedCmdListNil s)
+  then show ?case
+    by (meson red_cmd_list.RedCmdListNil)
+next
+  case (RedCmdListCons c s s'' cs s')
+
+  then have oneStep: "A,[],\<Lambda>',\<Gamma>,\<Omega> \<turnstile> \<langle>c,s\<rangle> \<rightarrow> s''"
+    by (metis Diff_cancel Int_empty_right map_le_refl red_cfg_dead_variables_cmd)
+
+
+  have freeVarCmdList: "free_var_cmdlist cs \<inter> (dom (map_of (snd \<Lambda>')) - dom (map_of (snd \<Lambda>))) = {}"
+    using RedCmdListCons.prems(3)
+    unfolding free_var_cmdlist.simps
+    by auto
+
+  have freeVarCmd: "free_var_cmd c \<inter> (dom (map_of (snd \<Lambda>')) - dom (map_of (snd \<Lambda>))) = {}"
+    using RedCmdListCons.prems(3)
+    unfolding free_var_cmdlist.simps
+    by auto
+
+  have oneStepCmd: "A,[],\<Lambda>,\<Gamma>,\<Omega> \<turnstile> \<langle>c,s\<rangle> \<rightarrow> s''"
+    by (rule red_cfg_dead_variables_cmd[OF oneStep assms(2) assms(3) freeVarCmd WhereClausesFreeVars])
+
+
+
+  have "A,[],\<Lambda>,\<Gamma>,\<Omega> \<turnstile> \<langle>cs,s''\<rangle> [\<rightarrow>] s'"
+    using RedCmdListCons(3) freeVarCmdList assms(2) MapLocal WhereClausesFreeVars
+    sorry (*Why doesn't this hold trivially? Shouldn't it directly follow from the implication?*)
+
+  
+    
+  then show ?case
+    using RedCmdListCons.IH RedCmdListCons.prems(2) RedCmdListCons.prems(3) assms(2) red_cmd_list.RedCmdListCons oneStepCmd by blast
+qed
+
+lemma red_cfg_dead_variables_cmdlist_onestep:
+  assumes oneStep: "A,[],\<Lambda>',\<Gamma>,\<Omega>,body \<turnstile>(Inl m, Normal ns) -n\<rightarrow> (m', s')" and
+          fstEq: "fst \<Lambda> = fst \<Lambda>'" and
+          MapLocal: "(map_of (snd \<Lambda>) \<subseteq>\<^sub>m map_of (snd \<Lambda>'))" and
+          NoDeadVariables: "free_var_cmdlist (node_to_block body ! m) \<inter> ((dom (map_of (snd \<Lambda>'))) - (dom (map_of (snd \<Lambda>)))) = {}" and
+          WhereClausesFreeVars: "\<And>x d cond. lookup_var_decl \<Lambda>' x = Some d \<Longrightarrow> snd d = Some cond \<Longrightarrow> free_var_expr cond \<inter> ((dom (map_of (snd \<Lambda>'))) - (dom (map_of (snd \<Lambda>)))) = {} "
+        shows   "A,[],\<Lambda>,\<Gamma>,\<Omega>,body \<turnstile>(Inl m, Normal ns) -n\<rightarrow> (m', s')"
+  using assms
+proof cases
+  case (RedNormalSucc cs ns' n')
+  have "A,[],\<Lambda>,\<Gamma>,\<Omega> \<turnstile> \<langle>cs,Normal ns\<rangle> [\<rightarrow>] Normal ns'"
+    apply (rule red_cfg_dead_variables_cmdlist[OF RedNormalSucc(4) fstEq MapLocal _ WhereClausesFreeVars])
+    using NoDeadVariables local.RedNormalSucc(3) by auto
+
+  then show ?thesis
+    using local.RedNormalSucc(1) local.RedNormalSucc(2) local.RedNormalSucc(3) local.RedNormalSucc(5) red_cfg.RedNormalSucc by blast
+next
+  case (RedNormalReturn cs ns')
+  have "A,[],\<Lambda>,\<Gamma>,\<Omega> \<turnstile> \<langle>cs,Normal ns\<rangle> [\<rightarrow>] Normal ns'"
+    apply (rule red_cfg_dead_variables_cmdlist[OF RedNormalReturn(4) fstEq MapLocal _ WhereClausesFreeVars])
+    using NoDeadVariables local.RedNormalReturn(3) by auto
+
+  then show ?thesis
+    using local.RedNormalReturn(1) local.RedNormalReturn(2) local.RedNormalReturn(3) local.RedNormalReturn(5) red_cfg.RedNormalReturn by blast
+next
+  case (RedFailure cs)
+  have "A,[],\<Lambda>,\<Gamma>,\<Omega> \<turnstile> \<langle>cs,Normal ns\<rangle> [\<rightarrow>] Failure"
+    apply (rule red_cfg_dead_variables_cmdlist[OF RedFailure(4) fstEq MapLocal _ WhereClausesFreeVars])
+    using NoDeadVariables local.RedFailure(3) by auto
+  then show ?thesis
+    using local.RedFailure(1) local.RedFailure(2) local.RedFailure(3) red_cfg.RedFailure by blast
+next
+  case (RedMagic cs)
+  have "A,[],\<Lambda>,\<Gamma>,\<Omega> \<turnstile> \<langle>cs,Normal ns\<rangle> [\<rightarrow>] Magic"
+    apply (rule red_cfg_dead_variables_cmdlist[OF RedMagic(4) fstEq MapLocal _ WhereClausesFreeVars])
+    using NoDeadVariables local.RedMagic(3) by auto
+  then show ?thesis
+    using local.RedMagic(1) local.RedMagic(2) local.RedMagic(3) red_cfg.RedMagic by blast
+qed
+
+lemma dom_map_of_append_pre_post:
+  assumes "map_of A \<subseteq>\<^sub>m map_of B" and
+          "dom (map_of A) \<inter> dom (map_of C) = {}"
+        shows "dom (map_of (D@B@C)) - dom (map_of (D@A@C)) = dom (map_of B) - dom (map_of A)"
+  using assms
+  apply (simp)
+  sorry
+
+lemma red_cfg_multi_dead_variables:
+  assumes RedCfg: "A,[],(constants @ global_vars, proc_args proc @ locals' @ proc_rets proc),\<Gamma>,\<Omega>,body \<turnstile>(Inl m, Normal ns) -n\<rightarrow>* (m', s')" and
+          MapLocal: "map_of locals \<subseteq>\<^sub>m map_of locals'" and
+          DomLocalInterRetsEmpty:   "dom (map_of locals') \<inter> dom (map_of (proc_rets proc)) = {}" and
+          NoDeadVariables: "\<forall>b\<in>set(node_to_block body). free_var_cmdlist b \<inter> (dom (map_of locals') - (dom (map_of locals))) = {}" and
+          WhereClausesFreeVars: "\<And>x d cond. lookup_var_decl (constants @ global_vars, proc_args proc @ locals' @ proc_rets proc) x = Some d \<Longrightarrow> snd d = Some cond \<Longrightarrow> free_var_expr cond \<inter> ((dom (map_of (snd (constants @ global_vars, proc_args proc @ locals' @ proc_rets proc)))) - (dom (map_of (snd (constants @ global_vars, proc_args proc @ locals @ proc_rets proc))))) = {} "
+        shows   "A,[],(constants @ global_vars, proc_args proc @ locals @ proc_rets proc),\<Gamma>,\<Omega>,body \<turnstile>(Inl m, Normal ns) -n\<rightarrow>* (m', s')"
+  using RedCfg WhereClausesFreeVars NoDeadVariables
+proof (induction rule: converse_rtranclp_induct2)
+  case refl
+  then show ?case
+    by simp
+next
+  case (step a b c d)
+  have restSteps: "A,[],(constants @ global_vars, proc_args proc @ locals @ proc_rets proc),\<Gamma>,\<Omega>,body \<turnstile>(c, d) -n\<rightarrow>* (m', s')"
+    using step.IH step.prems(1) step.prems(2) by blast
+  from step show ?case
+  proof (cases)
+    case (RedNormalSucc n cs ns ns' n')
+    have oneStepLocals':"A,[],(constants @ global_vars, proc_args proc @ locals' @ proc_rets proc),\<Gamma>,\<Omega>,body \<turnstile> (Inl n, Normal ns) -n\<rightarrow> (c, d)"
+      using local.RedNormalSucc(1) local.RedNormalSucc(2) step.hyps(1) by auto
+
+    have nInBody: "node_to_block body ! n \<in> set(node_to_block body)"
+      sorry
+
+
+    have "A,[],(constants @ global_vars, proc_args proc @ locals @ proc_rets proc),\<Gamma>,\<Omega>,body \<turnstile> (Inl n, Normal ns) -n\<rightarrow> (c, d)"
+      apply (rule red_cfg_dead_variables_cmdlist_onestep[OF oneStepLocals'])
+      apply (simp)
+      using DomLocalInterRetsEmpty MapLocal map_le_append_pre_post apply fastforce
+      using dom_map_of_append_pre_post nInBody NoDeadVariables
+      apply (smt (verit, ccfv_threshold) DomLocalInterRetsEmpty MapLocal disjoint_iff_not_equal domD domI map_le_def snd_eqD)
+      using WhereClausesFreeVars by auto
+    then show ?thesis
+      by (simp add: converse_rtranclp_into_rtranclp local.RedNormalSucc(1) local.RedNormalSucc(2) restSteps)
+  next
+    case (RedNormalReturn n cs ns ns')
+    have oneStepLocals':"A,[],(constants @ global_vars, proc_args proc @ locals' @ proc_rets proc),\<Gamma>,\<Omega>,body \<turnstile> (Inl n, Normal ns) -n\<rightarrow> (c, d)"
+      using local.RedNormalReturn(1) local.RedNormalReturn(2) step.hyps(1) by auto
+
+   have nInBody: "node_to_block body ! n \<in> set(node_to_block body)"
+     sorry
+
+   have "A,[],(constants @ global_vars, proc_args proc @ locals @ proc_rets proc),\<Gamma>,\<Omega>,body \<turnstile> (Inl n, Normal ns) -n\<rightarrow> (c, d)"
+      apply (rule red_cfg_dead_variables_cmdlist_onestep[OF oneStepLocals'])
+      apply (simp)
+      using DomLocalInterRetsEmpty MapLocal map_le_append_pre_post apply fastforce
+      using dom_map_of_append_pre_post nInBody NoDeadVariables
+      apply (smt (verit, ccfv_threshold) DomLocalInterRetsEmpty MapLocal disjoint_iff_not_equal domD domI map_le_def snd_eqD)
+      by (meson WhereClausesFreeVars)
+    then show ?thesis
+      by (simp add: converse_rtranclp_into_rtranclp local.RedNormalReturn(1) local.RedNormalReturn(2) restSteps)
+  next
+    case (RedFailure n cs ns)
+    have oneStepLocals':"A,[],(constants @ global_vars, proc_args proc @ locals' @ proc_rets proc),\<Gamma>,\<Omega>,body \<turnstile> (Inl n, Normal ns) -n\<rightarrow> (c, d)"
+      using local.RedFailure(1) local.RedFailure(2) step.hyps(1) by auto
+
+   have nInBody: "node_to_block body ! n \<in> set(node_to_block body)"
+     sorry
+
+   have "A,[],(constants @ global_vars, proc_args proc @ locals @ proc_rets proc),\<Gamma>,\<Omega>,body \<turnstile> (Inl n, Normal ns) -n\<rightarrow> (c, d)"
+      apply (rule red_cfg_dead_variables_cmdlist_onestep[OF oneStepLocals'])
+      apply (simp)
+      using DomLocalInterRetsEmpty MapLocal map_le_append_pre_post apply fastforce
+      using dom_map_of_append_pre_post nInBody NoDeadVariables
+      apply (smt (verit, ccfv_threshold) DomLocalInterRetsEmpty MapLocal disjoint_iff_not_equal domD domI map_le_def snd_eqD)
+      by (meson WhereClausesFreeVars)
+    then show ?thesis
+      by (simp add: converse_rtranclp_into_rtranclp local.RedFailure(1) local.RedFailure(2) restSteps)
+  next
+    case (RedMagic n cs ns)
+    have oneStepLocals':"A,[],(constants @ global_vars, proc_args proc @ locals' @ proc_rets proc),\<Gamma>,\<Omega>,body \<turnstile> (Inl n, Normal ns) -n\<rightarrow> (c, d)"
+      using local.RedMagic(1) local.RedMagic(2) step.hyps(1) by auto
+
+   have nInBody: "node_to_block body ! n \<in> set(node_to_block body)"
+     sorry
+
+   have "A,[],(constants @ global_vars, proc_args proc @ locals @ proc_rets proc),\<Gamma>,\<Omega>,body \<turnstile> (Inl n, Normal ns) -n\<rightarrow> (c, d)"
+      apply (rule red_cfg_dead_variables_cmdlist_onestep[OF oneStepLocals'])
+      apply (simp)
+      using DomLocalInterRetsEmpty MapLocal map_le_append_pre_post apply fastforce
+      using dom_map_of_append_pre_post nInBody NoDeadVariables
+      apply (smt (verit, ccfv_threshold) DomLocalInterRetsEmpty MapLocal disjoint_iff_not_equal domD domI map_le_def snd_eqD)
+      using WhereClausesFreeVars by auto
+    then show ?thesis
+      by (simp add: converse_rtranclp_into_rtranclp local.RedMagic(1) local.RedMagic(2) restSteps)
+  qed
+qed
+
+
+
+subsection \<open>Dead variables elimination lemma\<close>
+
+lemma elimination:
+  assumes proc_cor: "proc_is_correct A fun_decls constants global_vars axioms proc Semantics.proc_body_satisfies_spec" and
+          Body1: "proc_body proc = Some (locals, body)" and
+          Body2: "proc' = proc \<lparr>proc_body := Some (locals', body)\<rparr>" and
+          LocalVariables: "map_of locals \<subseteq>\<^sub>m map_of locals'" and 
+          FreeVarPres: "free_var_exprlist (proc_all_pres proc) \<inter> dom (map_of locals') - dom (map_of locals) = {}" and
+          FreeVarPosts: "free_var_exprlist (proc_checked_posts proc) \<inter> dom (map_of locals') - dom (map_of locals) = {}" and
+          DeadVariables: "\<forall>b\<in>set(node_to_block body). free_var_cmdlist b \<inter> (dom (map_of locals') - (dom (map_of locals))) = {}" and
+                 \<comment>\<open>The following assumption is needed to lift \<^term>\<open>map_of locals \<subseteq>\<^sub>m map_of locals'\<close>
+                    to the concatenation of all variables in the local state (arguments, locals, return variables)\<close>
+          DomLocalInterRetsEmpty: "dom (map_of locals') \<inter> dom (map_of (proc_rets proc)) = {}" and
+          WhereClausesFreeVars: "\<And>x d cond. lookup_var_decl (constants @ global_vars, proc_args proc @ locals' @ proc_rets proc) x = Some d \<Longrightarrow> snd d = Some cond \<Longrightarrow> free_var_expr cond \<inter> ((dom (map_of (snd (constants @ global_vars, proc_args proc @ locals' @ proc_rets proc)))) - (dom (map_of (snd (constants @ global_vars, proc_args proc @ locals @ proc_rets proc))))) = {} "
+        shows "proc_is_correct A fun_decls constants global_vars axioms proc' Semantics.proc_body_satisfies_spec"
+proof (simp add: Body2 del: proc_checked_posts.simps, (rule impI | rule allI)+)
+  fix \<Gamma> \<Omega> gs ls
+  assume  Atyp: "(\<forall>t. closed t \<longrightarrow> (\<exists>v. type_of_val A v = t)) \<and> (\<forall>v. closed (type_of_val A v))" and
+          FunWf:"fun_interp_wf A fun_decls \<Gamma>" and
+          ARenv: "list_all closed \<Omega> \<and> length \<Omega> = proc_ty_args proc" and
+          WfGlobal: "state_typ_wf A \<Omega> gs (constants @ global_vars)" and
+          WfLocal: "state_typ_wf A \<Omega> ls (proc_args proc @ locals' @ proc_rets proc)" and 
+          AxSat: "axioms_sat A (constants, []) \<Gamma>
+                      \<lparr>old_global_state = Map.empty, global_state = state_restriction gs constants, local_state = Map.empty,
+                      binder_state = Map.empty\<rparr> axioms"
+  show  "proc_body_satisfies_spec A [] (constants @ global_vars, proc_args proc @ locals' @ proc_rets proc) \<Gamma> \<Omega>
+        (map fst (proc_pres proc)) (proc_checked_posts (proc\<lparr>proc_body := Some (locals', body)\<rparr>)) body
+        \<lparr>old_global_state = gs, global_state = gs, local_state = ls, binder_state = Map.empty\<rparr>"
+    unfolding proc_body_satisfies_spec_def
+  proof ((rule impI | rule allI)+)
+    fix m' s'
+    assume ExprAllSat: "expr_all_sat A (constants @ global_vars, proc_args proc @ locals' @ proc_rets proc) \<Gamma> \<Omega>
+        \<lparr>old_global_state = gs, global_state = gs, local_state = ls, binder_state = Map.empty\<rparr> (map fst (proc_pres proc))" and
+           GoesTo: "A,[],(constants @ global_vars, proc_args proc @ locals' @ proc_rets proc),\<Gamma>,\<Omega>,body \<turnstile>(Inl (entry body),
+                                Normal \<lparr>old_global_state = gs, global_state = gs, local_state = ls, binder_state = Map.empty\<rparr>) -n\<rightarrow>* (m', s')"
+    show "valid_configuration A (constants @ global_vars, proc_args proc @ locals' @ proc_rets proc) \<Gamma> \<Omega>
+        (proc_checked_posts (proc\<lparr>proc_body := Some (locals', body)\<rparr>)) m' s'"
+      unfolding valid_configuration_def
+    proof -
+
+      have valid_proc: "valid_configuration A (constants @ global_vars, proc_args proc @ locals @ proc_rets proc) \<Gamma> \<Omega> ((proc_checked_posts proc)) m' s'"
+      proof (rule validConf [OF proc_cor Body1 Atyp FunWf ARenv WfGlobal])
+        show "state_typ_wf A \<Omega> ls (proc_args proc @ locals @ proc_rets proc)"
+          using state_typ_wf_map_le[OF WfLocal LocalVariables] DomLocalInterRetsEmpty
+          by blast
+      next
+        show "axioms_sat A (constants, []) \<Gamma> (global_to_nstate (state_restriction gs constants)) axioms"
+          using AxSat
+          by simp
+      next
+        show "expr_all_sat A (constants @ global_vars, proc_args proc @ locals @ proc_rets proc) \<Gamma> \<Omega>
+             \<lparr>old_global_state = gs, global_state = gs, local_state = ls, binder_state = Map.empty\<rparr> (proc_all_pres proc)"
+        proof -
+          have "expr_all_sat A (constants @ global_vars, proc_args proc @ locals' @ proc_rets proc) \<Gamma> \<Omega>
+               \<lparr>old_global_state = gs, global_state = gs, local_state = ls, binder_state = Map.empty\<rparr> (proc_all_pres proc)"
+            using ExprAllSat
+            by simp
+
+          thus "expr_all_sat A (constants @ global_vars, proc_args proc @ locals @ proc_rets proc) \<Gamma> \<Omega>
+             \<lparr>old_global_state = gs, global_state = gs, local_state = ls, binder_state = Map.empty\<rparr> (proc_all_pres proc)"
+            apply (rule expr_list_sat_dead_variables)
+            using LocalVariables FreeVarPres DomLocalInterRetsEmpty by blast
+        qed
+
+      next
+        show "A,[],(constants @ global_vars, proc_args proc @ locals @ proc_rets proc),\<Gamma>,\<Omega>,body \<turnstile>(Inl (entry body), Normal
+              \<lparr>old_global_state = gs, global_state = gs, local_state = ls, binder_state = Map.empty\<rparr>) -n\<rightarrow>* (m', s')"
+          by (rule red_cfg_multi_dead_variables[OF GoesTo LocalVariables DomLocalInterRetsEmpty DeadVariables WhereClausesFreeVars])
+      qed
+       
+       
+      hence notFailure: "s' \<noteq> Failure"
+        using valid_configuration_def by blast
+
+      have FinalConfig: "(is_final_config (m', s') \<longrightarrow> (\<forall>ns'. s' = Normal ns' \<longrightarrow> 
+                        expr_all_sat A (constants @ global_vars, proc_args proc @ locals' @ proc_rets proc) \<Gamma> \<Omega> ns' (proc_checked_posts (proc\<lparr>proc_body := Some (locals', body)\<rparr>))))" 
+            (is "?isFinal \<longrightarrow> (\<forall>ns'. ?isNormal ns' \<longrightarrow> ?Goal ns')")
+      proof ((rule impI | rule allI)+)
+        fix ns'
+        assume "?isFinal" and "?isNormal ns'" 
+        show "?Goal ns'"
+        proof -
+          
+          have EqPosts: "(proc_checked_posts proc) = (proc_checked_posts (proc\<lparr>proc_body := Some (locals', body)\<rparr>))"
+            sorry
+
+          have "expr_all_sat A (constants @ global_vars, proc_args proc @ locals @ proc_rets proc) \<Gamma> \<Omega> ns' (proc_checked_posts proc)"
+            using valid_proc 
+            unfolding valid_configuration_def
+            using \<open>is_final_config (m', s')\<close> \<open>s' = Normal ns'\<close> by blast
+
+
+          hence "expr_all_sat A (constants @ global_vars, proc_args proc @ locals' @ proc_rets proc) \<Gamma> \<Omega> ns' (proc_checked_posts proc)"
+            apply (rule expr_list_sat_dead_variables)
+            using LocalVariables FreeVarPosts DomLocalInterRetsEmpty by blast
+
+            
+
+          thus "expr_all_sat A (constants @ global_vars, proc_args proc @ locals' @ proc_rets proc) \<Gamma> \<Omega> ns' (proc_checked_posts (proc\<lparr>proc_body := Some (locals', body)\<rparr>))"
+            using EqPosts
+            by argo
+        qed
+      qed
+      thus "s' \<noteq> Failure \<and> (is_final_config (m', s') \<longrightarrow> (\<forall>ns'. s' = Normal ns' \<longrightarrow>
+            expr_all_sat A (constants @ global_vars, proc_args proc @ locals' @ proc_rets proc) \<Gamma> \<Omega> ns' (proc_checked_posts (proc\<lparr>proc_body := Some (locals', body)\<rparr>))))"
+        using notFailure by blast
+    qed
+  qed
+qed
 
 end
